lexer/lexer_spec_to_dfaScript.sml
@@ -5,28 +5,28 @@ val _ = new_theory "lexer_spec_to_dfa"
 
 val is_error_state_def = Define `
 is_error_state lex_spec =
-  EVERY (λ(regexp,action). is_regexp_empty regexp) lex_spec`;
+  EVERY (λ(regexp,action). regexp = CharSet {}) lex_spec`;
 
-val lex_spec_to_dfa_def = Define `
-lex_spec_to_dfa lex_spec = 
-  ((\(state,c). 
-    let state' = MAP (\(regexp,action). (deriv c regexp, action)) state in
-      if is_error_state state' then
-        NONE
-      else
-        SOME state'),
-   lex_spec,
-   (\state.
-     case FILTER (\(regexp,action). nullable regexp) state of
-       | (regexp,action)::_ => SOME action
-       | _ => NONE))`;
+val lex_spec_transition_def = Define `
+lex_spec_transition (state,c) =
+  let state' = MAP (\(regexp,action). (smart_deriv c regexp, action)) state in
+    if is_error_state state' then
+      NONE
+    else
+      SOME state'`;
+
+val lex_spec_finals_def = Define `
+lex_spec_finals state =
+  case FILTER (\(regexp,action). nullable regexp) state of
+     | (regexp,action)::_ => SOME action
+     | _ => NONE`;
 
 val lex_spec_action_lem = Q.prove (
 `n < LENGTH start_st ∧
- (FST (lex_spec_to_dfa lex_spec) (start_st,c) = SOME start_st') 
+ (lex_spec_transition (start_st,c) = SOME start_st') 
  ⇒
  (SND (EL n start_st) = SND (EL n start_st'))`,
-rw [LET_THM, lex_spec_to_dfa_def] >>
+rw [LET_THM, lex_spec_transition_def] >>
 rw [EL_MAP] >>
 cases_on `EL n start_st` >>
 rw []);
@@ -34,37 +34,37 @@ rw []);
 val lex_spec_trans_lem = Q.prove (
 `n < LENGTH start_st' ∧
  n < LENGTH start_st ∧
- (FST (lex_spec_to_dfa lex_spec) (start_st,c) = SOME start_st') ∧
+ (lex_spec_transition (start_st,c) = SOME start_st') ∧
  regexp_matches (FST (EL n start_st')) (MAP FST p)
  ⇒
  regexp_matches (FST (EL n start_st)) (STRING c (MAP FST p))`,
-rw [LET_THM, lex_spec_to_dfa_def] >>
+rw [LET_THM, lex_spec_transition_def] >>
 POP_ASSUM MP_TAC >>
 rw [EL_MAP] >>
 cases_on `EL n start_st` >>
-fs [regexp_matches_deriv, deriv_matches_def]);
+fs [regexp_matches_smart_deriv, smart_deriv_matches_def]);
 
 val lex_spec_trans_lem2 = Q.prove (
 `n' < n ∧
  n' < LENGTH start_st' ∧
  n' < LENGTH start_st ∧
- (FST (lex_spec_to_dfa lex_spec) (start_st,c) = SOME start_st') ∧
+ (lex_spec_transition (start_st,c) = SOME start_st') ∧
  ¬regexp_matches (FST (EL n' start_st')) (MAP FST p)
  ⇒
  ¬regexp_matches (FST (EL n' start_st)) (STRING c (MAP FST p))`,
-rw [LET_THM, lex_spec_to_dfa_def] >>
+rw [LET_THM, lex_spec_transition_def] >>
 POP_ASSUM MP_TAC >>
 rw [EL_MAP] >>
 cases_on `EL n' start_st` >>
-fs [regexp_matches_deriv, deriv_matches_def]);
+fs [regexp_matches_smart_deriv, smart_deriv_matches_def]);
 
 val path_to_spec = Q.prove (
 `!trans start_st end_st p.
   dfa_path trans start_st end_st p 
   ⇒
   !t.
-    (trans = FST (lex_spec_to_dfa lex_spec)) ∧
-    (SND (SND (lex_spec_to_dfa lex_spec)) end_st = SOME t)
+    (trans = lex_spec_transition) ∧
+    (lex_spec_finals end_st = SOME t)
     ⇒
     ∃n.
       n < LENGTH start_st ∧ (SND (EL n start_st) = t) ∧
@@ -72,7 +72,7 @@ val path_to_spec = Q.prove (
       (∀n'. n' < n ⇒ ¬regexp_matches (FST (EL n' start_st)) (MAP FST p))`,
 ho_match_mp_tac dfa_path_ind >>
 rw [LET_THM,dfa_path_def] >|
-[fs [lex_spec_to_dfa_def] >>
+[fs [lex_spec_transition_def, lex_spec_finals_def] >>
      cases_on `FILTER (λ(regexp,action). nullable regexp) end_st` >>
      fs [] >>
      PairCases_on `h`  >>
@@ -92,18 +92,22 @@ rw [LET_THM,dfa_path_def] >|
           PairCases_on `h` >>
           fs [] >>
           metis_tac [nullable_thm]],
- cases_on `FST (lex_spec_to_dfa lex_spec) (start_st,c)` >>
+ cases_on `lex_spec_transition (start_st,c)` >>
      fs [] >>
      rw [] >>
      res_tac >>
      fs [] >>
      rw [] >>
      `n < LENGTH start_st` 
-              by (fs [LET_THM,lex_spec_to_dfa_def] >>
+              by (fs [LET_THM,lex_spec_transition_def] >>
                   metis_tac [LENGTH_MAP]) >>
      qexists_tac `n` >>
      rw [] >>
      metis_tac [arithmeticTheory.LESS_TRANS, lex_spec_action_lem, lex_spec_trans_lem, lex_spec_trans_lem2]]);
+
+val lemma = Q.prove  (
+`!s. ~regexp_matches (CharSet {}) s`,
+rw [regexp_matches_def]);
 
 val spec_to_path = Q.prove (
 `∀n lex_spec l.
@@ -113,12 +117,12 @@ val spec_to_path = Q.prove (
   ⇒
   ∃p s.
     (l = MAP FST p) ∧
-    dfa_path (FST (lex_spec_to_dfa lex_spec)) (FST (SND (lex_spec_to_dfa lex_spec))) s p ∧
-    (SND (SND (lex_spec_to_dfa lex_spec)) s = SOME (SND (EL n lex_spec)))`,
+    dfa_path lex_spec_transition lex_spec s p ∧
+    (lex_spec_finals s = SOME (SND (EL n lex_spec)))`,
 induct_on `l` >>
 rw [] >|
 [qexists_tac `lex_spec` >>
-     rw [dfa_path_def, lex_spec_to_dfa_def, nullable_thm] >>
+     rw [dfa_path_def, lex_spec_transition_def, lex_spec_finals_def, nullable_thm] >>
      REPEAT (pop_assum mp_tac) >>
      Q.SPEC_TAC (`lex_spec`, `lex_spec`) >>
      induct_on `n` >>
@@ -135,26 +139,26 @@ rw [] >|
      `SUC n' < SUC n` by decide_tac >>
      metis_tac [EL, FST, HD, TL],
  `∀n'. n' < n ⇒
-         ¬deriv_matches (FST (EL n' (MAP (λ(regexp,action). (deriv h regexp,action)) lex_spec))) l`
+         ¬smart_deriv_matches (FST (EL n' (MAP (λ(regexp,action). (smart_deriv h regexp,action)) lex_spec))) l`
                by (rw [] >>
                    `n' < LENGTH lex_spec` by decide_tac >>
                    rw [EL_MAP, LENGTH_MAP] >>
-                   fs [deriv_matches_def, regexp_matches_deriv] >>
+                   fs [smart_deriv_matches_def, regexp_matches_smart_deriv] >>
                    cases_on  `EL n' lex_spec` >>
                    rw [] >>
                    metis_tac [FST]) >>
      qpat_assum `!n lex_spec. P n lex_spec` 
-            (MP_TAC o Q.SPECL [`n`, `THE ((FST (lex_spec_to_dfa lex_spec)) (lex_spec,h))`]) >>
-     rw [lex_spec_to_dfa_def, EL_MAP, LET_THM] >>
+            (MP_TAC o Q.SPECL [`n`, `THE (lex_spec_transition (lex_spec,h))`]) >>
+     rw [lex_spec_transition_def, lex_spec_finals_def, EL_MAP, LET_THM] >>
      cases_on `EL n lex_spec` >>
-     fs [regexp_matches_deriv, deriv_matches_def] >|
+     fs [regexp_matches_smart_deriv, smart_deriv_matches_def] >|
      [fs [is_error_state_def, EVERY_MAP] >>
           fs [EVERY_EL] >>
           res_tac >>
           cases_on `EL n lex_spec` >>
           fs [] >>
           rw [] >>
-          metis_tac [regexp_matches_deriv, regexp_empty_thm],
+          metis_tac [regexp_matches_smart_deriv, lemma],
       res_tac >>
           rw [] >>
           cases_on `FILTER (λ(regexp,action). nullable regexp) s` >>
@@ -162,23 +166,21 @@ rw [] >|
           PairCases_on `h'` >>
           fs [] >>
           rw [] >>
-          qexists_tac `(h,MAP (λ(regexp,action). (deriv h regexp,action)) lex_spec)::p` >>
+          qexists_tac `(h,MAP (λ(regexp,action). (smart_deriv h regexp,action)) lex_spec)::p` >>
           qexists_tac `s` >>
-          rw [dfa_path_def]]]);
+          rw [dfa_path_def,lex_spec_transition_def] >>
+          fs []]]);
 
 val lex_spec_to_dfa_correct = Q.store_thm ("lex_spec_to_dfa_correct",
 `!lex_spec.
-  dfa_correct lex_spec 
-      (FST (lex_spec_to_dfa lex_spec))
-      (SND (SND (lex_spec_to_dfa lex_spec)))
-      (FST (SND (lex_spec_to_dfa lex_spec)))`,
+  dfa_correct lex_spec lex_spec_transition lex_spec_finals lex_spec`,
 rw [dfa_correct_def] >>
 eq_tac >>
 rw [] >|
 [imp_res_tac path_to_spec >>
-     fs [lex_spec_to_dfa_def],
+     fs [],
  imp_res_tac spec_to_path >>
-     fs [lex_spec_to_dfa_def] >>
+     fs [] >>
      metis_tac []]);
 
 val _ = export_theory ();
